Qed a boring spec for `errors.Unwrap`

new/proof/errors.v
@@ -8,14 +8,30 @@ Local Set Default Proof Using "All".
 #[global] Instance : IsPkgInit (iProp Σ) errors := define_is_pkg_init True%I.
 #[global] Instance : GetIsPkgInitWf (iProp Σ) errors := build_get_is_pkg_init_wf.
 
+Definition is_unwrappable (err : error.t) : iProp Σ :=
+  □(match err with
+  | interface.nil => True
+  | interface.ok ii =>
+      if decide (method_set ii.(interface.ty) !! "Unwrap"%go = Some $ go.Signature [] false [go.error]) then
+        ({{{ True }}}
+           #(methods ii.(interface.ty) "Unwrap" ii.(interface.v)) #()
+         {{{ err, RET #(interface.ok err); True }}})%I
+      else True%I
+  end).
+
 Lemma wp_Unwrap (err : error.t) :
-  {{{ True }}}
+  {{{ is_unwrappable err }}}
     @! errors.Unwrap #err
-  {{{ RET #err; True }}}.
+  {{{ (err' : error.t), RET #err'; True }}}.
 Proof.
-  wp_start. wp_auto. destruct err.
-  2:{ wp_auto. wp_end. }
-  (* TODO: cases for err being not nil. *)
-Admitted.
+  wp_start as "#Hunwrap". wp_auto. destruct err; simpl.
+  2:{ (* err is nil *) wp_auto. wp_end. }
+  destruct go.type_set_contains eqn:Hhas_unwrap.
+  - (* err has an Unwrap function *)
+    rewrite /go.type_set_contains go.is_underlying /= in Hhas_unwrap.
+    rewrite andb_true_r in Hhas_unwrap. rewrite bool_decide_eq_true in Hhas_unwrap.
+    rewrite decide_True //. wp_auto. wp_apply "Hunwrap" as "% _". wp_end.
+  - wp_auto. wp_end.
+Qed.
 
 End wps.
